vcalyx/coq/Arith.v
@@ -1,0 +1,28 @@
+From stdpp Require Import
+     base
+     numbers.
+Require Import VCalyx.Value.
+Definition value_lift_binop (f: N -> N -> N) : value -> value -> value :=
+  fun u v =>
+    match u, v with
+    | Bot, _
+    | _, Bot => Bot
+    | V u, V v => V (f u v)
+    | Top, _
+    | _, Top => Top
+    end.
+
+Definition value_lt : value -> value -> value :=
+  value_lift_binop (fun n m => bool_to_N (N.ltb n m)).
+
+Definition value_or : value -> value -> value :=
+  value_lift_binop N.lor.
+
+Definition value_add : value -> value -> value :=
+  value_lift_binop N.add.
+
+Definition value_div_quotient : value -> value -> value :=
+  value_lift_binop N.div.
+
+Definition value_div_remainder : value -> value -> value :=
+  value_lift_binop (fun a b => (N.div_eucl a b).2).
