vcalyx/coq/Value.v
@@ -1,0 +1,35 @@
+From stdpp Require Import
+     base
+     strings
+     numbers.
+Require Import Coq.Classes.EquivDec.
+Require Import VCalyx.Exception.
+
+Inductive value := 
+(* Top: more than 1 assignment to this port has occurred *)
+| Top 
+(* If only 1 assignment has occurred, this value is in port.in *)
+| V (val: N)
+(* Bottom: no assignment to this port has occurred *)
+| Bot.
+Scheme Equality for value.
+#[export] Instance value_EqDec : EqDec value eq :=
+  value_eq_dec.
+
+Definition expect_V (v: value) : exn N :=
+  match v with
+  | V val => mret val
+  | _ => err "expect_V"
+  end.
+
+Definition is_one (v: value) :=
+  v ==b (V 1%N).
+
+Definition is_nonzero (v: value) :=
+  v <>b (V 0%N).
+
+Definition bool_to_N (b: bool) : N :=
+  if b then 1%N else 0%N.
+
+Definition bool_to_value (b: bool) : value :=
+  V (bool_to_N b).
